src/Common/Notations.v
@@ -4,6 +4,13 @@ Reserved Notation "\ x , e" (at level 78).
 Reserved Notation "\ ! , e" (at level 78).
 Reserved Infix "⊓" (at level 80).
 Reserved Infix "⊔" (at level 80).
+Reserved Infix "##" (at level 60, right associativity).
 Reserved Infix "=s" (at level 70, no associativity).
 Reserved Infix "=b" (at level 70, no associativity).
 Reserved Notation "s ~= [ ch ]" (at level 70, no associativity).
+Reserved Infix "=?" (at level 70).
+Reserved Infix "<=?" (at level 70).
+Reserved Infix "<?" (at level 70).
+Reserved Infix "?=" (at level 70).
+Reserved Notation "'⊤'".
+Reserved Notation "'⊥'".
